theories/Pretty.v
@@ -264,4 +264,4 @@ Definition print_as_program (t : term) :=
 
 Definition let_test := let binding := TermBind (VarDecl "y" (Ty_Builtin DefaultUniInteger)) (Constant (ValueOf DefaultUniInteger 1)) in
  Let [binding] (Apply (LamAbs "x" (Ty_Builtin DefaultUniInteger) (Var "x")) (Var "y")).
-Eval cbv in print_as_program let_test.
+(* Eval cbv in print_as_program let_test. *)
